WIP: input_top multiple ports

dataplane/Examples/Input_top.thy
@@ -5,160 +5,65 @@ imports
   "../Utils"
 begin 
 
-
-corec input_top where
-  "input_top c inps = (case inps of
-    LNil \<Rightarrow> drop_cap c \<oslash>
-  | LCons xs lxs \<Rightarrow>
-     push 
-     (Write (input_top (Cap (time c + 1) (out c)) lxs) (trace (STR ''Managing caps'') None) (Inl (Inl \<lparr> cons = [], inte = [(out c, time c, -1), (out c, time c + 1, 1)], prod = case xs of [] => [] | _ \<Rightarrow> [(out c, time c, length xs)]\<rparr>)))
-      (1 :: 1) (map (\<lambda> x. (x, c)) xs))"
-
-lemma step_input_top_elim:
-  assumes "step io (input_top c inps) op'"
-  obtains
-    x xs where "io = Out (Some 1) (Inr (x, time c))" "lhd inps = xs" "hd xs = x" "inps \<noteq> LNil" "xs \<noteq> []"
-    "op' = writes (Write (input_top (Cap (time c + 1) (out c)) (ltl inps)) None (Inl (Inl \<lparr> cons = [], inte = [(out c, time c, -1), (out c, time c + 1, 1)], prod = [(out c, time c, length xs)]\<rparr>))) (Some 1) (map (\<lambda> x. Inr (x, time c)) (tl xs))"
-  | "io = Out None (Inl (Inl \<lparr>cons = [], inte = [(out c, time c, - 1), (out c, time c + 1, 1)], prod = []\<rparr>)) " "inps \<noteq> LNil" "lhd inps = []" "op' = input_top (Cap (time c + 1) (out c)) (ltl inps)"
-  | "inps = LNil" "io = Out None (Inl (Inl \<lparr> cons = [], inte = [(out c, time c, -1)], prod = [] \<rparr>))" "op' = \<oslash>"
-  using assms apply -
-  apply atomize_elim
-  apply (subst (asm) input_top.code)
-  apply (simp split: llist.splits)
-  apply force
-  subgoal for xs lxs
-    apply hypsubst_thin
-    apply (cases io; simp)
-    subgoal
-      using step_writes_reads_buf_empty by fastforce
-    subgoal for p x
-      apply hypsubst_thin
-      apply (cases xs; simp)
-      subgoal
-        by auto
-      subgoal
-        apply (drule step_Out_writes)
-        apply (auto simp add: comp_def)
-        done
-      done
-    subgoal
-      apply (cases xs; simp)
-      apply force
-      apply (drule step_Out_writes)
-      apply auto
-      done
-    done
-  done
-
-lemma step_input_top_Out_Some_intro[intro]:
-  "inps = LCons xs inps' \<Longrightarrow>
-   xs = x # xs' \<Longrightarrow>
-   op = writes (Write (input_top (Cap (time c + 1) (out c)) inps') None (Inl (Inl \<lparr> cons = [], inte = [(out c, time c, -1), (out c, time c + 1, 1)], prod = [(out c, time c, length xs)]\<rparr>))) (Some 1) (map (\<lambda> x. Inr (x, time c)) xs') \<Longrightarrow>
-   step (Out (Some 1) (Inr (x, time c))) (input_top c inps) op"
-  apply (subst input_top.code)
-  apply (auto simp add: comp_def)
-  done
-
-lemma step_input_top_Out_None_intro[intro]:
-  "inps = LCons [] inps' \<Longrightarrow> 
-   step (Out None (Inl (Inl \<lparr> cons = [], inte = [(out c, time c, -1), (out c, Suc (time c), 1)], prod = []\<rparr>))) (input_top c inps) (input_top (Cap (Suc (time c)) (out c)) inps')"
-  apply (subst input_top.code)
-  apply (auto simp add: comp_def)
-  done
-
-lemma ldropWhile_LCons_lfinite_ltakeWhile:
-  "ldropWhile ((=) []) inps = LCons (x # xs) inps' \<Longrightarrow> lfinite (ltakeWhile ((=) []) inps)"
-  by (metis ldropWhile_eq_LNil_iff lfinite_ltakeWhile llist.simps(2))
-
-lemma ldropWhile_steps_input_top:
-  "lfinite (ltakeWhile ((=) []) inps) \<Longrightarrow>
-   ldropWhile ((=) []) inps = LCons (x # xs) inps' \<Longrightarrow>
-   steps (map (\<lambda> t. Out None (Inl (Inl \<lparr> cons = [], inte = [(out c, t, -1), (out c, Suc t, 1)], prod = []\<rparr>))) [time c..<time c + the_enat (llength (ltakeWhile ((=) []) inps))])
-  (input_top c inps) (input_top (Cap (time c + the_enat (llength (ltakeWhile ((=) []) inps))) (out c)) (LCons (x # xs) inps'))"
-  apply (induct "ltakeWhile ((=) []) inps"  arbitrary: c inps rule: lfinite_induct)
-  subgoal for inps c
-    apply (cases "ltakeWhile ((=) []) inps"; simp)
-    apply (metis ldropWhile_simps(1,2) ltakeWhile_simps(2) neq_LNil_conv)
-    done
-  subgoal premises prems for inps c
-    using prems(1,2,4-) apply -
-    apply (cases inps; simp split: if_splits; hypsubst)
-    subgoal for z lxs
-      apply (rule steps_intro[where xs="map (\<lambda>t. Out None (Inl (Inl \<lparr>cons = [], inte = [(out c, t, - 1), (out c, Suc t, 1)], prod = []\<rparr>))) [Suc (time c)..<time c + the_enat (eSuc (llength (ltakeWhile ((=) []) lxs)))]"])
-      apply (rule step_input_top_Out_None_intro)
-      apply (rule refl)+
-      defer
-      subgoal
-        apply simp
-        apply (subst map_eq_Cons_conv)
-        apply auto
-        apply (intro exI conjI[rotated])
-        apply (rule refl)
-        apply (rule upt_conv_Cons)
-        apply (metis dataflow_topology_from_tree.le_plus(1) impossible_Cons le_neq_implies_less length_list_of_conv_the_enat lfinite.simps list_of_LCons llength_LCons nat_add_left_cancel_le)
-        done
-      subgoal
-        apply (subst (1 2) the_enat_eSuc)
-        using llength_eq_infty_conv_lfinite apply blast
-        using prems(3)[where c="Cap (time c + 1) (out c)" and inps=lxs] apply -
-        apply (simp split: if_splits)
-        done
-      done
-    done
-  done
-
-abbreviation "ex1 \<equiv> Logic (input_top (Cap 0 (1 :: 1)) (LCons [Suc 0, 3] (LCons [9] LNil))) :: (2, 1, (1, _) shared_state + 'c, nat \<times> _) dataflow_tree"
-(* 
-value [GHC] "eval 20 (compile_dataflow ex1)"
- *)
-(*value [GHC] "cfilter ((\<noteq>) []) (eval 20 (compile_dataflow (Comp [ (0, 0) \<mapsto> (0, 0) ] ex1 (Logic \<I>))))" *)
-
-(* value [GHC] "eval 17 (dataflow_op True init_subgraph (input_top (Cap (0 :: nat) 0) (LCons [Suc 0, 2, 3, 9] (LCons [8, 1, 0] LNil))))"
-value [GHC] "eval 5 (dataflow_op True init_subgraph (input_top (Cap (0 :: nat) 0) (LCons [Suc 0] (LNil))))"
- *)
-
-
-(* value [GHC] "eval 20 (compile_dataflow ex13)"
-
-value [GHC] "eval 20 (input_op 0 (LCons [Suc 0, 3] (LCons [] (LCons [9] (LCons [9] LNil)))))"
- *)
-
-abbreviation "ex13 \<equiv> Logic (input_top (Cap 0 (1 :: 1)) (LCons [Suc 0, 3] (LCons [] (LCons [9] (LCons [9] LNil))))) :: (2, 1, (1, _) shared_state + 'c, nat \<times> _) dataflow_tree"
-
-corec input_op :: "nat \<Rightarrow> 'a buf llist \<Rightarrow> (1, 1, 'a \<times> nat) op" where
-  "input_op n inps = (case ldropWhile ((=) []) inps of
-     LNil \<Rightarrow> \<oslash>
-   | LCons (x # xs) lxs \<Rightarrow> Write (input_op (n + the_enat (llength (ltakeWhile ((=) []) inps))) (LCons xs lxs)) 1 (x, n + the_enat (llength (ltakeWhile ((=) []) inps))))"
+corec input_op where
+  "input_op n inps = Choice (cimage (\<lambda> p. case ldropWhile ((=) []) (inps p) of
+     LCons (x # xs) lxs \<Rightarrow> 
+     Write 
+     (input_op (n(p := n p + the_enat (llength (ltakeWhile ((=) []) (inps p))))) (inps (p := LCons xs lxs)))
+       p (x, n p + the_enat (llength (ltakeWhile ((=) []) (inps p)))))
+      (cfilter (\<lambda> p. ldropWhile ((=) []) (inps p) \<noteq> LNil) c\<UU>))"
 
 lemma step_input_op_elim:
   assumes "step io (input_op n inps) op"
-  obtains x xs inps' where "io = Out 1 (x, n + the_enat (llength (ltakeWhile ((=) []) inps)))" "ldropWhile ((=) []) inps = LCons (x # xs) inps'" "op = input_op (n + the_enat (llength (ltakeWhile ((=) []) inps))) (LCons xs inps')"
+  obtains p x xs lxs where "io = Out p (x, n p + the_enat (llength (ltakeWhile ((=) []) (inps p))))" "ldropWhile ((=) []) (inps p) = LCons (x # xs) lxs"
+   "op = input_op (n (p := n p + the_enat (llength (ltakeWhile ((=) []) (inps p))))) (inps(p := LCons xs lxs))" "p \<notin> defaults"
   using assms apply -
   apply atomize_elim
   apply (subst (asm) input_op.code)
-  apply (simp split: llist.splits list.splits)
-  using ldropWhile_LConsD apply fast
+  apply (clarsimp split: llist.splits list.splits)
+  apply (metis (full_types) ldropWhile_LConsD)
   apply auto
   done
 
 lemma step_input_op_Out_intro[intro]:
-  "inps = LCons (x # xs) lxs \<Longrightarrow>
-   ys = LCons xs lxs \<Longrightarrow>
-   step (Out 1 (x, n)) (input_op n inps) (input_op n ys)"
+  "inps p = LCons (x # xs) lxs \<Longrightarrow>
+   ys = inps(p := LCons xs lxs) \<Longrightarrow>
+   p \<notin> defaults \<Longrightarrow>
+   step (Out p (x, n p)) (input_op n inps) (input_op n ys)"
   apply (subst input_op.code)
-  apply (auto split: llist.splits)
+  apply (clarsimp split: llist.splits)
+  apply (rule SC)
+   apply (rule cimage_eqI[rotated])
+    apply force
+   apply (rule refl)
+  apply simp
+  apply force
+  done
+
+lemma step_input_op_Out_intro2[intro]:
+  "ldropWhile ((=) []) (inps p) = LCons (x # xs) lxs \<Longrightarrow>
+   p \<notin> defaults \<Longrightarrow>
+   step (Out p (x, (n p) + the_enat (llength (ltakeWhile ((=) []) (inps p))))) (input_op n inps) (input_op (n (p := n p + the_enat (llength (ltakeWhile ((=) []) (inps p))))) (inps(p := LCons xs lxs)))"
+  apply (subst input_op.code)
+  apply (clarsimp split: llist.splits)
+  apply (rule SC)
+   apply (rule cimage_eqI[rotated])
+    apply force
+   apply (rule refl)
+  apply simp
+  apply force
   done
 
 lemma step_input_op_not_Tau[simp]:
   "\<not> step Tau (input_op n inps) op"
   apply (subst input_op.code)
-  apply (auto split: llist.splits list.splits dest: ldropWhile_LConsD)
+  apply (auto split: llist.splits list.splits dest!: ldropWhile_LConsD)
   done
 
 lemma step_input_op_not_Inp[simp]:
   "\<not> step (Inp p x) (input_op n inps) op"
   apply (subst input_op.code)
-  apply (auto split: llist.splits list.splits dest: ldropWhile_LConsD)
+  apply (auto split: llist.splits list.splits dest!: ldropWhile_LConsD)
   done
 
 lemma wstep_input_op_simp[simp]:
@@ -178,178 +83,15 @@ lemma wstep_input_op_simp[simp]:
     done
   done
 
-lemma input_op_LCons_Nil:
-  "input_op i (LCons [] lxs) = input_op (Suc i) lxs"
-  apply (cases "llength (ltakeWhile ((=) []) lxs) \<noteq> \<infinity>")
-  subgoal
-    apply (subst (1 2) input_op.code)
-    apply (simp split: llist.splits list.splits)
-    apply (subst (1 2) the_enat_eSuc)
-    apply simp_all
-    done
-  subgoal
-    apply (subst (1 2) input_op.code)
-    apply (simp split: llist.splits list.splits)
-    apply (meson ldropWhile_LCons_lfinite_ltakeWhile llength_eq_infty_conv_lfinite)
-    done
-  done
 
-lemma input_op_LNil:
-  "input_op i LNil = \<oslash>"
-  apply (subst input_op.code)
-  apply simp
-  done
-
-lemma dataflow_op_input_top_input_op:
-  "edges sg = (\<lambda> _. []) \<Longrightarrow>
-   dataflow_op sg (map_op (case_option (Inl nid) (\<lambda>p. Inr (nid, p))) (case_option (Inl nid) (\<lambda>p. Inr (nid, p))) (input_top (Cap i (1 :: 1)) inps)) \<approx>
-   map_op (\<lambda> p. (nid, p)) (\<lambda> p. (nid, p)) (input_op i inps)"
-proof (coinduction arbitrary: inps i sg rule: wbisim_coinduct)
-  case SIM1
-  then show ?case
-    apply -
-    apply (elim step_map_op_elim step_dataflow_op_elim step_input_top_elim conjE; simp; hypsubst_thin)
-    subgoal for nida op'' io' op''a xa xs
-      apply (cases inps)
-      apply simp
-      subgoal for xs lxs
-        apply (cases xs; simp)
-        subgoal for x xs'
-          apply (intro exI conjI)
-          apply (rule step_wstep)
-          apply fastforce
-          apply hypsubst_thin
-          apply (rule wbcr_base)
-          apply (rule exI)
-          apply (rule exI)
-          apply (rule exI[of _ "sg\<lparr> lo_pt := (lo_pt sg) @ extract_progress nid (edges sg) \<lparr>cons = [], inte = [], prod = [(1, i, 1)]\<rparr> \<rparr>"])
-          apply (intro conjI[rotated])
-          apply simp
-          apply (rule refl)
-          apply (subst (2) input_top.code)
-          apply (simp add: comp_def split: if_splits)
-          apply (cases xs')
-          subgoal
-            apply simp
-            apply (subst (1 2) dataflow_op.code)
-            apply (auto simp add: extract_progress_def split: if_splits option.splits)
-            done
-          subgoal
-            sorry
-(*             apply simp
-            apply (rule box_equals) 
-            defer
-            apply (rule dataflow_writes_extract_progress_from_push[symmetric, where p="1 :: 1", simplified])
-            apply (rule refl)
-            apply (rule dataflow_writes_extract_progress_from_push[symmetric, where p="1 :: 1", simplified])
-            apply (rule refl)
-            apply (clarsimp simp add: extract_progress_def split: option.splits) 
-            done*)
-          done
-        done
-      done
-    subgoal 
-      apply (cases inps; simp)
-      subgoal for x lxs
-        apply (intro exI conjI)
-        apply (subst input_op_LCons_Nil)
-        apply (rule rtranclp.intros(1))
-        apply (rule wbcr_base)
-        apply (rule exI)
-        apply (rule exI)
-        apply (rule exI[of _ "sg\<lparr> lo_pt := (lo_pt sg) @ extract_progress nid (edges sg) \<lparr>cons = [], inte = [(1, i, - 1), (1, Suc i, 1)], prod = []\<rparr> \<rparr>"])
-        apply (intro conjI[rotated])
-        defer
-        apply (rule refl)+
-        apply simp_all
-        done
-      done
-    subgoal
-      apply (auto simp add: dataflow_op_end_op input_op_LNil)
-      done
-    done
-next
-  case SIM2
-  then show ?case
-    apply -
-    apply (elim step_map_op_elim step_input_op_elim conjE; simp; hypsubst_thin)
-    subgoal for io' op'' x xs inps'
-      apply (intro exI conjI)
-      unfolding wstep_def
-      apply simp
-      apply (rule relcomppI[rotated])
-      apply (rule relcomppI[rotated])
-      apply (rule rtranclp.intros(1))
-      apply (rule step_Out_dataflow_op_Out_Inr_intro)
-      apply (rule step_map_op[where f="case_option (Inl nid) (\<lambda>p. Inr (nid, 1))" and g="case_option (Inl nid) (\<lambda>p. Inr (nid, 1))"])
-      apply simp_all
-      apply (rule step_input_top_Out_Some_intro[where c="Cap (i + the_enat (llength (ltakeWhile ((=) []) inps))) 1" and xs="x # xs"])
-      apply assumption
-      apply (rule refl)+
-      apply simp
-      apply (rule relpowp_imp_rtranclp) 
-      apply (rule steps_Tau_dataflow_op_Out_Inl_intro[where nid=nid and sg=sg and xs="map (\<lambda> t. \<lparr> cons = [], inte = [(1, t, -1), (1, Suc t, 1)], prod = [] \<rparr>) ([i..< i + (the_enat (llength (ltakeWhile ((=) []) inps)))])" ])
-      apply (rule steps_map_op)
-           apply simp
-      defer
-      apply (rule ldropWhile_steps_input_top[where  c="Cap i 1", simplified])
-      apply (meson ldropWhile_LCons_lfinite_ltakeWhile)
-      apply simp
-      apply simp
-      apply (rule refl)+
-      apply (intro conjI wbcr_base)
-      apply (rule exI[of _ "LCons xs inps'"])
-      apply (rule exI[of _ "i + the_enat (llength (ltakeWhile ((=) []) inps))"])
-      apply (rule exI[of _ "sg\<lparr> lo_pt := (lo_pt sg) @ extract_progress nid (edges sg) \<lparr>cons = [], inte = concat (map (\<lambda> t. [(1, t, -1), (1, Suc t, 1)]) [i..< i + (the_enat (llength (ltakeWhile ((=) []) inps)))]), prod = [(1, i, 1)]\<rparr> \<rparr>"])
-      apply (intro conjI)
-      apply simp
-         apply (clarsimp simp add: extract_progress_def split: option.splits)
-      oops
-(*       apply (subst dataflow_writes_extract_progress_from_push[where p="1 :: 1", simplified])
-      apply (rule refl)
-      apply (clarsimp simp add: extract_progress_def split: option.splits)
-      apply simp_all
-      apply (cases xs)
-      subgoal
-        apply (subst (2) input_top.code)
-        apply (simp add: comp_def)
-        apply (subst (1 2) dataflow_extract_progress_from_push[simplified])
-        apply (clarsimp simp add: extract_progress_def split: option.splits)
-        apply (rule arg_cong2[where f=dataflow_op])
-        apply simp_all
-        apply (cases sg; simp)
-        apply (simp add: map_concat)
-        apply (rule arg_cong[where f=concat])
-        apply (rule map_cong)
-        apply simp_all
-        done
-      subgoal
-        apply (subst (2) input_top.code)
-        apply (simp add: comp_def)
-        apply (subst (1 2) dataflow_writes_extract_progress_from_push[simplified])
-        apply (clarsimp simp add: extract_progress_def split: option.splits)
-        apply (rule refl)+
-        apply force
-        apply (rule arg_cong2[where f=dataflow_op])
-        apply simp_all
-        apply (cases sg; simp)
-        apply (simp add: map_concat extract_progress_def)
-        apply (simp add: map_concat)
-        apply (rule arg_cong[where f=concat])
-        apply (rule map_cong)
-        apply simp_all
-        done
-      done
-    done
-qed *)
-
+(* 
 lemma compile_dataflow_input_top_input_op:
   "(compile_dataflow (Logic (input_top (Cap i 1) inps)) :: (1 \<times> 1, 1 \<times> 1, 'b \<times> nat) op) \<approx> map_op (\<lambda> p. (1, p)) (\<lambda> p. (1, p)) (input_op i inps)"
   unfolding compile_dataflow_def Let_def
   apply (simp split: prod.splits)
   apply (intro conjI allI impI)
   subgoal for su op
-    oops(* 
+    oops
     using dataflow_op_input_top_input_op[where sg="init_subgraph su", simplified, where i=i and inps=inps] apply -
     apply (drule meta_mp)
     subgoal
@@ -387,148 +129,113 @@ lemma compile_dataflow_input_top_input_op:
 lemma input_top_correctness:
   "wtraced (compile_dataflow (Logic (input_top (Cap i 1) inps)) :: (1 \<times> 1, 1 \<times> 1, 'b \<times> nat) op) ios \<Longrightarrow>
    ios = (lmap (\<lambda> (n, t). VOut (1, 0) (n, t)) (lconcat (lmap (\<lambda> (xs, t). map (\<lambda> n. (n, t)) xs) (lzip inps (iterates Suc i)))))"
-  oops(* 
-  apply (drule wbisim_wtraced[OF compile_dataflow_input_top_input_op])
-  apply (coinduction arbitrary: ios inps i)
-  subgoal for ios inps i
-    apply (cases ios)
-    subgoal
-      apply (erule wtraced.cases)
-      apply simp_all
-      apply (subst (asm) wfinished_map_op)
-      apply simp_all
-      apply (erule wfinished.cases)
-      subgoal for ops
-       apply (clarsimp simp add: input_op.code lnull_def split: llist.splits list.splits prod.splits)
-        apply (metis (full_types) ldropWhile_eq_LNil_iff lset_lzipD1)
-        apply (metis (full_types) ldropWhile_LConsD)
-        done
-      subgoal for op
-       apply (clarsimp simp add: input_op.code lnull_def split: llist.splits list.splits prod.splits)
-        apply (metis (full_types) ldropWhile_LConsD)
-        done
-      done
-    subgoal for io ios'
-      apply simp
-      apply (erule wtraced.cases)
-      apply simp_all
-      apply hypsubst_thin
-      apply (elim wstep_map_op_elim)
-      apply (subst (asm) wstep_input_op_simp)
-      apply force
-      apply (elim step_input_op_elim)
-      apply (cases io; simp)
-      apply hypsubst_thin
-      apply safe
-      subgoal premises prems
-        using prems(2-) apply -
-        unfolding lnull_def
-        apply (auto simp add: lset_lzip split: prod.splits)
-        apply (metis (full_types) in_lset_conv_lnth ldropWhile_eq_LNil_iff llist.distinct(1))
-        done
-      subgoal premises prems for op' io' op'' x xs inps' a b
-        using prems(2-) apply -
-        apply (subst lhd_lconcat_lmap_zip)
-        apply simp_all
-        apply (meson ldropWhile_LCons_lfinite_ltakeWhile)
-        done
-      subgoal for op' io' op'' x xs inps' a b
-        apply (intro conjI[rotated] exI)
-        apply assumption
-        apply simp
-        subgoal premises prems
-          using prems(2) apply -
-          apply (rule llist.map_cong)
-          apply simp_all
-          apply (rule ltl_lconcat_lmap_zip)
-          apply simp_all
-          apply (meson ldropWhile_LCons_lfinite_ltakeWhile)
-          done
-        done
-      done
-    done
-  done *)
+  oops
 
-corec nd_input_top where
-  "nd_input_top c ints prds inps = choice2 
-  (case inps of
-    LNil \<Rightarrow> Write \<oslash> None (Inl (Inl \<lparr> cons = [], inte = ints, prod = prds @ [(1, time c, -1)]\<rparr>))
-  | LCons xs lxs \<Rightarrow> push (Silent (nd_input_top (Cap (time c + 1) (1 :: 1)) (ints @ [(1, time c, -1), (1, time c + 1, 1)]) (prds @ [(1, time c, length xs)]) lxs)) (1 :: 1) (map (\<lambda> x. (x, c)) xs))
-  (Write (nd_input_top c [] [] inps) None (Inl (Inl \<lparr> cons = [], inte = ints, prod = prds\<rparr>)))"
+abbreviation "send_output op p x \<equiv> Write op (Some p) (Inr x)"
+abbreviation "send_progress op st \<equiv> Write op None (Inl (Inl st))"
 
-lemma step_nd_input_top_elim:
-  assumes "step io (nd_input_top c ints prds inps) op'"
+abbreviation "obtain_progress os \<equiv> (os\<lparr> consu := [], inter := [], produ := [] \<rparr>, \<lparr> cons = consu os, inte = inter os, prod = produ os\<rparr>)"
+
+
+corec input_top where
+  "input_top os inps = 
+   choice2 
+     (Choice (cimage (\<lambda> p. 
+     choice2
+       (case inps p of
+         LNil \<Rightarrow> Silent (input_top (deactivate_port os p) inps)
+       | LCons batch lxs \<Rightarrow> (let last_t = stash os p in 
+                             case obtain_cap os last_t p of
+                               (_, None) \<Rightarrow> Silent \<oslash>
+                             | (os', Some cap) \<Rightarrow>
+                                let os'' = produce os' cap batch in
+                                let os''' = delay_cap os'' cap 1 in
+                                Silent (input_top os''' (inps(p := lxs)))))
+       (case get_output os p of
+         (os', None) \<Rightarrow> Silent (input_top os' inps)
+       | (os', Some x) \<Rightarrow> send_output (input_top os' inps) p x)
+     ) c\<UU>))
+    (let (os', st) = obtain_progress os in
+     send_progress (input_top os' inps) st)"
+
+thm step_id_op_cases
+
+lemma step_input_top_elim:
+  assumes "step io (input_top os inps) op'"
   obtains
-    x xs lxs where "io = Out (Some 1) (Inr (x, time c))" "inps = LCons (x # xs) lxs"
-    "op' = push (Silent (nd_input_top (Cap (time c + 1) 1) (ints @ [(1, time c, -1), (1, time c + 1, 1)]) (prds @ [(1, time c, length (x # xs))]) lxs)) (1 :: 1) (map (\<lambda> x. (x, c)) xs)"
-  | lxs where "io = Tau" "inps = LCons [] lxs" "op' = nd_input_top (Cap (time c + 1) 1) (ints @ [(1, time c, -1), (1, time c + 1, 1)]) (prds @ [(1, time c, 0)]) lxs"
-  | "io = Out None (Inl (Inl \<lparr> cons = [], inte = ints, prod = prds @ [(1, time c, -1)]\<rparr>))" "inps = LNil" "op' = \<oslash>"
-  | "io = Out None (Inl (Inl \<lparr> cons = [], inte = ints, prod = prds\<rparr>))" "op' = nd_input_top c [] [] inps"
+    batch lxs p last_t os' os'' os''' cap where "io = Tau" "inps p = LCons batch lxs" "last_t = stash os p"
+    "obtain_cap os last_t p = (os', Some cap)" "os'' = produce os' cap batch"
+    "os''' = delay_cap os'' cap 1" "op' = input_top os''' (inps(p := lxs))" "p \<notin> defaults"
+  | batch lxs p last_t os' where "io = Tau" "inps p = LCons batch lxs" "last_t = stash os p"
+    "obtain_cap os last_t p = (os', None)" "op' = \<oslash>" "p \<notin> defaults"
+  | p where "io = Tau" "inps p = LNil" "op' = input_top (deactivate_port os p) inps" "p \<notin> defaults"
+  | p os' where "io = Tau" "get_output os p = (os', None)" "op' = input_top os' inps" "p \<notin> defaults"
+  | p os' x where "io = Out (Some p) (Inr x)" "get_output os p = (os', Some x)"
+    "op' = input_top os' inps" "p \<notin> defaults"
+  | os' st where "io = Out None (Inl (Inl st))" "obtain_progress os = (os', st)"
+    "op' = input_top os' inps"
   using assms apply -
   apply atomize_elim
-  apply (subst (asm) nd_input_top.code)
-  apply (simp split: llist.splits)
-   apply force
-  subgoal for xs lxs
-    apply hypsubst_thin
-    apply (cases io; simp)
-    subgoal for p x
-      apply (cases xs; simp)
-      subgoal
-        by auto
-      subgoal
-        by (auto simp add: comp_def writes_Cons_simp)
+  apply (subst (asm) input_top.code)
+  apply (cases io)
+  subgoal
+    by (auto split: llist.splits prod.splits option.splits)
+  subgoal
+    by (auto split: llist.splits prod.splits option.splits)
+  subgoal
+    apply (clarsimp simp flip: cin.rep_eq del: disjCI split: llist.splits prod.splits option.splits if_splits; hypsubst_thin?)
+    apply (elim disjE)
+    subgoal
+      apply (clarsimp simp flip: cin.rep_eq del: disjCI split: llist.splits prod.splits option.splits if_splits; hypsubst_thin?)
+           apply force+
       done
     subgoal
-      apply (cases xs; simp)
-      by (auto simp add: comp_def writes_Cons_simp)
-    subgoal
-      apply (cases xs; simp)
-      by (auto simp add: comp_def writes_Cons_simp)
+      apply (auto simp flip: cin.rep_eq del: disjCI split: llist.splits prod.splits option.splits if_splits; hypsubst_thin?)
+      done
     done
-  done
-
-
-lemma step_nd_input_top_Out_Some_intro[intro!]:
-  "inps = LCons (x # xs) inps' \<Longrightarrow>
-   op = push (Silent (nd_input_top (Cap (time c + 1) 1) (ints @ [(1, time c, -1), (1, time c + 1, 1)]) (prds @ [(1, time c, int (length (x # xs)))]) inps')) (1 :: 1) (map (\<lambda> x. (x, c)) xs) \<Longrightarrow>
-   io = Out (Some 1) (Inr (x, time c)) \<Longrightarrow>
-   step io (nd_input_top c ints prds inps) op"
-  apply (subst nd_input_top.code)
-  apply (auto simp add: comp_def)
-  done
-
-lemma step_nd_input_top_Tau_intro[intro!]:
-  "inps = LCons [] inps' \<Longrightarrow> 
-   op = nd_input_top (Cap (time c + 1) 1) (ints @ [(1, time c, -1), (1, time c + 1, 1)]) (prds @ [(1, time c, 0)]) inps' \<Longrightarrow>
-   step Tau (nd_input_top c ints prds inps) op"
-  apply (subst nd_input_top.code)
-  apply (auto simp add: comp_def)
-  done
-
-lemma step_nd_input_top_Out_None_intro[intro]:
-  "op = nd_input_top c [] [] inps \<Longrightarrow>
-   step (Out None (Inl (Inl \<lparr> cons = [], inte = ints, prod = prds\<rparr>))) (nd_input_top c ints prds inps) op"
-  apply (subst nd_input_top.code)
-  apply (auto simp add: comp_def)
-  done
-
-
-lemma step_nd_input_top_Out_None_end_intro[intro]:
-  "op = \<oslash> \<Longrightarrow>
-   inps = LNil \<Longrightarrow>
-   step (Out None (Inl (Inl \<lparr> cons = [], inte = ints, prod = prds @ [(1, time c, -1)]\<rparr>))) (nd_input_top c ints prds inps) op"
-  apply (subst nd_input_top.code)
-  apply (auto simp add: comp_def)
   done
 
 (* 
-lemma ldropWhile_steps_nd_input_top:
+lemma step_input_top_Out_Some_intro[intro!]:
+  "inps = LCons (x # xs) inps' \<Longrightarrow>
+   op = push (Silent (input_top (Cap (time c + 1) 1) (ints @ [(1, time c, -1), (1, time c + 1, 1)]) (prds @ [(1, time c, int (length (x # xs)))]) inps')) (1 :: 1) (map (\<lambda> x. (x, c)) xs) \<Longrightarrow>
+   io = Out (Some 1) (Inr (x, time c)) \<Longrightarrow>
+   step io (input_top c ints prds inps) op"
+  apply (subst input_top.code)
+  apply (auto simp add: comp_def)
+  done
+
+lemma step_input_top_Tau_intro[intro!]:
+  "inps = LCons [] inps' \<Longrightarrow> 
+   op = input_top (Cap (time c + 1) 1) (ints @ [(1, time c, -1), (1, time c + 1, 1)]) (prds @ [(1, time c, 0)]) inps' \<Longrightarrow>
+   step Tau (input_top c ints prds inps) op"
+  apply (subst input_top.code)
+  apply (auto simp add: comp_def)
+  done
+
+lemma step_input_top_Out_None_intro[intro]:
+  "op = input_top c [] [] inps \<Longrightarrow>
+   step (Out None (Inl (Inl \<lparr> cons = [], inte = ints, prod = prds\<rparr>))) (input_top c ints prds inps) op"
+  apply (subst input_top.code)
+  apply (auto simp add: comp_def)
+  done
+
+
+lemma step_input_top_Out_None_end_intro[intro]:
+  "op = \<oslash> \<Longrightarrow>
+   inps = LNil \<Longrightarrow>
+   step (Out None (Inl (Inl \<lparr> cons = [], inte = ints, prod = prds @ [(1, time c, -1)]\<rparr>))) (input_top c ints prds inps) op"
+  apply (subst input_top.code)
+  apply (auto simp add: comp_def)
+  done
+ *)
+(* 
+lemma ldropWhile_steps_input_top:
   "lfinite (ltakeWhile ((=) []) inps) \<Longrightarrow>
    ldropWhile ((=) []) inps = LCons (x # xs) inps' \<Longrightarrow>
    ints' = concat (map (\<lambda> t. [(out c, t, -1), (out c, Suc t, 1)]) [time c..<time c + the_enat (llength (ltakeWhile ((=) []) inps))]) \<Longrightarrow>
    steps (replicate (the_enat (llength (ltakeWhile ((=) []) inps))) Tau)
-  (nd_input_top c ints prds inps) (nd_input_top (Cap (time c + the_enat (llength (ltakeWhile ((=) []) inps))) (out c)) (ints @ ints') prds (LCons (x # xs) inps'))"
+  (input_top c ints prds inps) (input_top (Cap (time c + the_enat (llength (ltakeWhile ((=) []) inps))) (out c)) (ints @ ints') prds (LCons (x # xs) inps'))"
   apply (induct "ltakeWhile ((=) []) inps"  arbitrary: c inps ints ints' rule: lfinite_induct)
   subgoal for inps c
     apply (cases "ltakeWhile ((=) []) inps"; simp; hypsubst_thin)
@@ -539,7 +246,7 @@ lemma ldropWhile_steps_nd_input_top:
     apply (cases inps; simp split: if_splits; hypsubst)
     subgoal for z lxs
       apply (rule steps_intro[where xs="replicate (the_enat (llength (ltakeWhile ((=) []) lxs))) Tau"])
-      apply (rule step_nd_input_top_Tau_intro)
+      apply (rule step_input_top_Tau_intro)
          apply (rule refl)+
       defer
       subgoal
@@ -557,7 +264,7 @@ lemma ldropWhile_steps_nd_input_top:
          defer
          apply simp
         apply (simp del: upt_Suc)
-        apply (rule arg_cong3[where f="nd_input_top (Cap (Suc (dataflow_topology_from_tree.followed_by (time c) (the_enat (llength (ltakeWhile ((=) []) lxs))))) (out c))"])
+        apply (rule arg_cong3[where f="input_top (Cap (Suc (dataflow_topology_from_tree.followed_by (time c) (the_enat (llength (ltakeWhile ((=) []) lxs))))) (out c))"])
           apply simp_all
         apply (intro impI)
         apply (subst (2) upt_conv_Cons)
@@ -567,62 +274,12 @@ lemma ldropWhile_steps_nd_input_top:
     done
   done *)
 
-(* FIXME: move me *)
-lemma input_op_LCons_write_simp:
-  "input_op i (LCons xs lxs) = writes (input_op (Suc i) lxs) 1 (map (\<lambda> x. (x, i)) xs)"
-  apply (induct xs arbitrary: i lxs)
-  apply (simp add: input_op_LCons_Nil)
-  subgoal for x xs i lxs
-    apply (simp add: writes_Cons_simp)
-    apply (subst input_op.code)
-    apply simp
-    done
-  done
 
-lemma bisim_writes_cong:
-  "op1 ~ op2 \<Longrightarrow>
-   writes op1 p xs ~ writes op2 p xs"
-  sorry
-
-lemma wbisim_writes_cong:
-  "op1 \<approx> op2 \<Longrightarrow>
-   writes op1 p xs \<approx> writes op2 p xs"
-  sorry
-
-lemma wbisim_Silent_cong:
-  "op1 \<approx> op2 \<Longrightarrow>
-   Silent op1 \<approx> op2"
-  sorry
-
-lemma step_bisim:
-  "(\<forall> io op'. step io op1 op' \<longleftrightarrow> step io op2 op') \<Longrightarrow>
-   op1 ~ op2"
-  sorry
-
-lemma Choice_singleton_bisim_alt:
-  "op1 ~ op2 \<Longrightarrow>
-   Choice {|op1|} ~ op2"
-  sorry
-
-lemma dataflow_op_wbisim_cong:
-  "op1 \<approx> op2 \<Longrightarrow>
-   dataflow_op sg op1 \<approx> dataflow_op sg op2"
-  sorry
-
-lemma dataflow_writes_comm:
-  "dataflow_op sg (writes op (Inr p) (map (\<lambda> x. Inr (f x)) xs)) ~ writes (dataflow_op sg op) p (map f xs)"
-  sorry
-
-lemma dataflow_Silent_comm:
-  "dataflow_op sg (Silent op) ~ Silent (dataflow_op sg op)"
-  sorry
-
-abbreviation "inp_top c ints prds inps \<equiv> map_op (case_option (Inl (0 :: 2)) (\<lambda> p. Inr (0, (p :: 1)))) (case_option (Inl (0 :: 2)) (\<lambda> p. Inr (0, (p :: 1)))) (nd_input_top c ints prds inps)"
+(* 
+abbreviation "inp_top c ints prds inps \<equiv> map_op (case_option (Inl (0 :: 2)) (\<lambda> p. Inr (0, (p :: 1)))) (case_option (Inl (0 :: 2)) (\<lambda> p. Inr (0, (p :: 1)))) (input_top c ints prds inps)"
 abbreviation "id_top buf \<equiv> map_op (case_option (Inl (1 :: 2)) (\<lambda> p. Inr (1, (p :: 1)))) (case_option (Inl (1 :: 2)) (\<lambda> p. Inr (1, (p :: 1)))) (id_op buf)"
 
-term "\<UU>"
-
-lemma dataflow_op_nd_input_top_input_op:
+lemma dataflow_op_input_top_input_op:
   "inrbufs1 = buf1 (Inr (1, 1)) \<Longrightarrow>
    \<forall> x \<in> set inrbufs1. is_Inr x \<Longrightarrow>
    inrbufs2 = buf2 (Some 1) \<Longrightarrow>
@@ -633,7 +290,7 @@ lemma dataflow_op_nd_input_top_input_op:
    lconcat (lmap (\<lambda> (xs, t). map (\<lambda> n. (n, t)) xs) (lzip inps1 (iterates Suc j))) \<Longrightarrow>
    edges sg = (\<lambda> _. []) \<Longrightarrow>
    dataflow_op sg ((map_op (case_sum id id) (case_sum id id) (comp_op [Inr (0 :: 2, 1 :: 1) \<mapsto> Inr (1, 1)] buf1 (inp_top (Cap i (1 :: 1)) ints prds inps2) (id_top buf2)))) \<approx>
-   dataflow_op sg (map_op (case_option (Inl 1) (\<lambda>p. Inr (1, p))) (case_option (Inl 1) (\<lambda>p. Inr (1, p))) (nd_input_top (Cap j (1 :: 1)) ints prds inps1))"
+   dataflow_op sg (map_op (case_option (Inl 1) (\<lambda>p. Inr (1, p))) (case_option (Inl 1) (\<lambda>p. Inr (1, p))) (input_top (Cap j (1 :: 1)) ints prds inps1))"
 proof (coinduction arbitrary: inps1 inps2 i j buf1 buf2 ints prds sg rule: weakBisimWeakUptoBisimCong)
   case SIM1
   then show ?case 
@@ -641,7 +298,7 @@ proof (coinduction arbitrary: inps1 inps2 i j buf1 buf2 ints prds sg rule: weakB
     unfolding wsim_def
     apply safe
     subgoal for io op1'
-      apply (elim step_map_op_elim step_dataflow_op_elim step_nd_input_top_elim step_comp_op_elim step_id_op_cases conjE; simp split: if_splits option.splits; hypsubst_thin)
+      apply (elim step_map_op_elim step_dataflow_op_elim step_input_top_elim step_comp_op_elim step_id_op_cases conjE; simp split: if_splits option.splits; hypsubst_thin)
       defer
       subgoal for op'' io' op''a p op1' q io'a op''b xa xs lxs
        apply (intro exI conjI)
@@ -649,27 +306,81 @@ proof (coinduction arbitrary: inps1 inps2 i j buf1 buf2 ints prds sg rule: weakB
     apply (simp add: comp_def)
         apply (intro relcomppI)
         defer
+        oops
+ *)
+
+fun input_list where
+  "input_list t [] = []"
+| "input_list t (xs # xss) = (map (\<lambda> x. (x, t)) xs) @ input_list (t + 1) xss"
 
 
-end
-lemma dataflow_op_nd_input_top_input_op:
+
+lemma ldropWhile_lshift:
+  "x \<in> set xs \<Longrightarrow>
+   \<not> P x \<Longrightarrow>
+   ldropWhile P (xs @@- lxs) = dropWhile P xs @@- lxs"
+  apply (induct xs)
+   apply auto
+  done
+
+
+lemma dataflow_op_input_top_input_op:
   "edges sg = (\<lambda> _. []) \<Longrightarrow>
-   dataflow_op sg (map_op (case_option (Inl nid) (\<lambda>p. Inr (nid, p))) (case_option (Inl nid) (\<lambda>p. Inr (nid, p))) (nd_input_top (Cap i (1 :: 1)) ints prds inps)) \<approx>
-   map_op (\<lambda> p. (nid, p)) (\<lambda> p. (nid, p)) (input_op i inps)"
-proof (coinduction arbitrary: inps i ints prds sg rule: weakBisimWeakUptoBisimCong)
+   (\<forall> p. input_list (t p) (xs p) = outpu os p) \<Longrightarrow>
+   dataflow_op sg (map_op (case_option (Inl nid) (\<lambda>p. Inr (nid, p))) (case_option (Inl nid) (\<lambda>p. Inr (nid, p))) (input_top (os\<lparr> stash := (\<lambda> p. t p + length (xs p)) \<rparr>) inps)) \<approx>
+   map_op (\<lambda> p. (nid, p)) (\<lambda> p. (nid, p)) (input_op t (\<lambda> p. xs p @@- inps p ))"
+proof (coinduction arbitrary: inps t rule: weakBisimWeakUptoBisimCong)
   case SIM1
   then show ?case 
     apply -
     unfolding wsim_def
     apply safe
     subgoal for io op1'
-    apply (elim step_map_op_elim step_dataflow_op_elim step_nd_input_top_elim conjE; simp; hypsubst_thin)
-    subgoal for nida op'' io' op''a xa xs lxs
+    apply (elim step_map_op_elim step_dataflow_op_elim step_input_top_elim conjE; simp split: list.splits; hypsubst_thin)
+      subgoal for nida p op'' x io' op''a os' xs
+        apply (cases x)
+        subgoal for y t'
+          apply hypsubst_thin
+          apply (drule spec[of _ p])
+          apply simp
       apply (intro exI conjI)
        apply (rule step_wstep)
        apply (rule step_map_op)
-       apply (rule step_input_op_Out_intro)
-        apply (rule refl)+
+          apply (rule step_input_op_Out_intro2[where p=p and x=y])
+             apply (subst ldropWhile_lshift)
+               defer
+               defer
+          defer
+             apply assumption
+            apply simp
+            defer
+            apply (intro relcomppI)
+          defer
+      apply (rule wb_upto_b_base)
+      apply (intro exI conjI[rotated])
+          defer
+                  apply (rule refl)+
+              defer
+          defer
+
+end
+      defer
+           apply assumption
+              apply simp
+          apply (intro conjI)
+               apply (rule refl)+
+              apply (drule spec[of _ p])
+              apply (simp add: lconcat_correct)
+
+
+
+          find_theorems Coinductive_List.lconcat ltakeWhile
+
+
+
+
+
+end
       apply simp
       apply (simp add: comp_def)
       apply (intro relcomppI)
@@ -746,7 +457,7 @@ end
       apply (rule step_bisim)
       apply safe
       subgoal
-    apply (elim step_map_op_elim step_dataflow_op_elim step_nd_input_top_elim conjE; simp; hypsubst_thin)
+    apply (elim step_map_op_elim step_dataflow_op_elim step_input_top_elim conjE; simp; hypsubst_thin)
         sledgehammer
 
       find_theorems writes bisim
@@ -797,7 +508,7 @@ end
 
       find_theorems writes map_op
 
-      apply (subst (2) nd_input_top.code)
+      apply (subst (2) input_top.code)
       apply (auto split: list.splits)
 
 end
@@ -845,7 +556,7 @@ next
          apply (rule steps_map_op)
          apply (rule refl)+
       defer
-      apply (rule ldropWhile_steps_nd_input_top[where  c="Cap i 1", simplified])
+      apply (rule ldropWhile_steps_input_top[where  c="Cap i 1", simplified])
             apply (meson ldropWhile_LCons_lfinite_ltakeWhile)
       apply assumption+
            apply (rule refl)+
@@ -854,7 +565,7 @@ next
       apply (rule step_Out_dataflow_op_Out_Inr_intro)
       apply (rule step_map_op[where f="case_option (Inl nid) (\<lambda>p. Inr (nid, 1))" and g="case_option (Inl nid) (\<lambda>p. Inr (nid, 1))"])
       apply simp_all
-      apply (rule step_nd_input_top_Out_Some_intro)
+      apply (rule step_input_top_Out_Some_intro)
       apply (rule refl)+
        apply simp_all
       done
